modified move; still proving

ATL.v
@@ -7,32 +7,27 @@ Require Export FunctionalExtensionality.
 Parameter State : Set.
 Parameter Player : Set.
 Parameter Observable : Set.
-
+Parameter Move : Set.
 Parameter beq_player : Player -> Player -> bool.
 
 
-Definition move_number : Set := State -> Player -> nat.
-
-Definition move {m:move_number} (q:State) (p:Player) :Set := nat.
-
-Definition move_vec {m:move_number} (q: State)  := forall (p:Player), @move m q p.
+Definition move_vec (q: State) := forall (p:Player), Move.
 
 Definition observation := State -> Observable.
 
-Definition delta {m:move_number} := forall (q:State), @move_vec m q -> State.
+Definition delta := forall (q:State), move_vec q -> State.
 
 Record CGS : Set := mkRat
                       {
                         size: nat;
                         lp:list Player;
-                        m:move_number;
                         o:observation;
-                        d:@delta m
+                        d:@delta
                        }.
 
 (* TODO: consider limiting coalitions to lp. *)
 
-Definition succ (g:CGS) (q q':State) := exists mv:@move_vec g.(m) q, q'=g.(d) q mv.
+Definition succ (g:CGS) (q q':State) := exists mv:move_vec q, q'=g.(d) q mv.
 
 Fixpoint computation_property_fix (g:CGS) (l:list State) : Prop :=
   match l with
@@ -161,9 +156,7 @@ Definition computation_prefix
 
 Check computation_prefix.
 
-Definition strategy (g:CGS) (p:Player) : Set := forall (q:State) (l:computation g q), (@move g.(m) (last (proj1_sig l) q) p).
-
-Definition strat_zero (g:CGS) (p:Player) : strategy g p := fun (q:State) => fun (l:computation g q) => 0.
+Definition strategy (g:CGS) (p:Player) : Set := forall (q:State) (l:computation g q), Move.
 
 Definition coalition : Type := Player -> bool.
 
@@ -188,17 +181,16 @@ Definition coal_intersection (c1 c2: coalition) : coalition :=
 
 Definition strategy_set (g:CGS) (c:coalition) : Set := forall (p:Player), c p = true -> strategy g p.
 
-Definition ss_zero (g:CGS) (c:coalition) : strategy_set g c := fun (p:Player) (H: (c p = true)) => strat_zero g p.
-
 Definition outcomes (g:CGS) (q:State) (c:coalition) (ss:strategy_set g c) (l: computation g q) : Prop
 :=
   forall (i:nat)
          (p:Player)
          (H: c p = true)
-         (m:move_vec (last (proj1_sig (computation_prefix g q l i)) q)),
+         (m:move_vec (nth i (proj1_sig l) q)),
     let x := computation_prefix g q l i in
-    m p = ss p H q x
-    -> g.(d) (last (proj1_sig x) q) m = (last (proj1_sig x) q).
+    m p = ss p H q x ->
+    S i  < (length (proj1_sig l)) ->
+    g.(d) (nth i (proj1_sig l) q) m = (nth (i+1) (proj1_sig l) q).
 
 
 Inductive sentence : Type :=
@@ -230,35 +222,36 @@ Check forall  (g:CGS) (q:State) (c: coalition),
       forall (l:computation g q),
         outcomes g q c ss l.
 
+Variable not_helper : CGS -> State -> sentence -> Prop.
 
-(* Inductive verifiesI: CGS -> State -> sentence -> Prop := *)
-(* | verifiesObs: forall (g: CGS) (q: State) (a: Observable), *)
-(*     g.(o) q = a -> verifiesI g q (obs a) *)
-(* | verifiesNot: forall (g: CGS) (q: State) (phi: sentence), *)
-(*     ~(verifiesI g q phi) -> *)
-(*     verifiesI g q (!! phi) *)
-(* | verifiesAnd: forall (g: CGS) (q: State) (phi1 phi2: sentence), *)
-(*     verifiesI g q phi1 -> *)
-(*     verifiesI g q phi2 -> *)
-(*     verifiesI g q (phi1 //\\ phi2) *)
-(* | verifiesPossibleNext: forall (g: CGS) (q: State) (phi: sentence) (c:coalition), *)
-(*     (exists (ss:strategy_set g c), *)
-(*       forall (l:computation g q), *)
-(*         outcomes g q c ss l -> *)
-(*         verifiesI g (nth 1 (proj1_sig l) q) phi) -> *)
-(*     verifiesI g q (<<c>>o phi) *)
-(* | verifiesPossibleOnce: forall (g: CGS) (q: State) (phi: sentence) (c:coalition), *)
-(*     (exists (ss:strategy_set g c), *)
-(*         forall (l:computation g q), *)
-(*           outcomes g q c ss l -> *)
-(*           (exists n:nat, verifiesI g (nth n (proj1_sig l) q) phi)) -> *)
-(*     verifiesI g q (<<c>>^ phi) *)
-(* | verifiesPossibleAlways: forall (g: CGS) (q: State) (phi: sentence) (c:coalition), *)
-(*     (exists (ss:strategy_set g c), *)
-(*         forall (l:computation g q), *)
-(*           outcomes g q c ss l -> *)
-(*           (forall n:nat, verifiesI g (nth n (proj1_sig l) q) phi)) -> *)
-(*     verifiesI g q (<<c>>^ phi). *)
+Inductive verifiesI: CGS -> State -> sentence -> Prop :=
+| verifiesObs: forall (g: CGS) (q: State) (a: Observable),
+    g.(o) q = a -> verifiesI g q (obs a)
+| verifiesNot: forall (g: CGS) (q: State) (phi: sentence),
+    ~ not_helper g q phi ->
+    verifiesI g q (!! phi)
+| verifiesAnd: forall (g: CGS) (q: State) (phi1 phi2: sentence),
+    verifiesI g q phi1 ->
+    verifiesI g q phi2 ->
+    verifiesI g q (phi1 //\\ phi2)
+| verifiesPossibleNext: forall (g: CGS) (q: State) (phi: sentence) (c:coalition),
+    (exists (ss:strategy_set g c),
+      forall (l:computation g q),
+        outcomes g q c ss l ->
+        verifiesI g (nth 1 (proj1_sig l) q) phi) ->
+    verifiesI g q (<<c>>o phi)
+| verifiesPossibleOnce: forall (g: CGS) (q: State) (phi: sentence) (c:coalition),
+    (exists (ss:strategy_set g c),
+        forall (l:computation g q),
+          outcomes g q c ss l ->
+          (exists n:nat, verifiesI g (nth n (proj1_sig l) q) phi)) ->
+    verifiesI g q (<<c>>^ phi)
+| verifiesPossibleAlways: forall (g: CGS) (q: State) (phi: sentence) (c:coalition),
+    (exists (ss:strategy_set g c),
+        forall (l:computation g q),
+          outcomes g q c ss l ->
+          (forall n:nat, verifiesI g (nth n (proj1_sig l) q) phi)) ->
+    verifiesI g q (<<c>>^ phi).
  
 
     
@@ -271,23 +264,22 @@ Fixpoint verifies (g:CGS) (q:State) (phi:sentence) :Prop :=
   | a \\// b => (verifies g q a) \/ (verifies g q b)
   | <<c>>o a => forall (l:computation g q),
       exists (ss:strategy_set g c),
-        outcomes g q c ss l
-        /\ (verifies g (nth 1 (proj1_sig l) q) a)
+        outcomes g q c ss l ->
+        (verifies g (nth 1 (proj1_sig l) q) a)
   | <<c>>^ a => forall (l:computation g q),
-      exists (ss:strategy_set g c),
-        outcomes g q c ss l
-        /\ exists (n:nat),
-          (verifies g (nth n (proj1_sig l) q) a)
+      exists (n:nat) (ss:strategy_set g c),
+        outcomes g q c ss l ->
+        (verifies g (nth n (proj1_sig l) q) a)
   | <<c>># a => forall (l:computation g q) (n:nat),
       exists (ss:strategy_set g c),
-        outcomes g q c ss l
-        /\ (verifies g (nth n (proj1_sig l) q) a)
+        outcomes g q c ss l ->
+        (verifies g (nth n (proj1_sig l) q) a)
   | <<c>> a %% b => forall (l:computation g q),
-      exists (ss:strategy_set g c) (n:nat),
-        outcomes g q c ss l
-        /\ (verifies g (nth n (proj1_sig l) q) b)
+      exists (n:nat) (ss:strategy_set g c),
+        outcomes g q c ss l ->
+        ((verifies g (nth n (proj1_sig l) q) b)
         /\ forall (m:nat),
-            m < n -> (verifies g (nth m (proj1_sig l) q) a)
+            m < n -> (verifies g (nth m (proj1_sig l) q) a))
   end.
 
 Definition invariant (g1 g2:CGS) : Prop := forall (phi:sentence) (q:State),
@@ -307,6 +299,11 @@ Proof.
   - reflexivity.
   - reflexivity.
 Qed.
+
+Theorem lnot_lnot : forall g q phi, verifies g q (!! (!! phi)) -> verifies g q phi.
+Proof.
+  simpl. intros. apply NNPP. apply H.
+Qed.
   
 Axiom d_sentence : forall (g:CGS) (q:State) (phi:sentence), decidable (verifies g q phi).
 
@@ -315,7 +312,9 @@ Theorem coalition_complement_once_always : forall (g:CGS) (q:State) (phi:sentenc
 Proof.
   intros g q.
   assert (F: forall c phi, verifies g q (<<c>>^ phi) -> verifies g q (!! ([[c]]# ( !! phi)))).
-  {simpl. unfold not. intros.
+  { simpl. intros.
+    apply ex_not_not_all.
+    
     assert (P: computation_property g q (q::nil)).
     {
       unfold computation_property. split. 
@@ -323,9 +322,41 @@ Proof.
       - reflexivity.
     }
     pose (l := (exist (computation_property g q) (q::nil) P) : (computation g q)).
-    destruct (H l), H1, H2. destruct (H0 l x0), H3. apply H4 in H2. apply H2.
+    exists l.
+    apply ex_not_not_all.
+    exists 0.
+    apply all_not_not_ex.
+    unfold not. intros.
+    apply H0.
+    unfold outcomes. intros. simpl in H3. destruct i.
+    + simpl in H3. inversion H3. inversion H5.
+    + inversion H3. inversion H5.
+    + simpl. destruct (H l). induction x.
+      * destruct H1. apply H1. unfold outcomes. intros. inversion H4. inversion H6.
+      * apply IHx. destruct H1. exists x0. intros. apply H1 in H2.
+        assert (proj1_sig l = (q::nil)).
+        {
+          unfold proj1_sig. unfold l. reflexivity.
+        }
+        assert (forall m:nat, nth (S m) (proj1_sig l) q = nth m (proj1_sig l) q).
+        {
+          intros. induction m.
+          - reflexivity.
+          - symmetry. apply nth_overflow. simpl. assert (forall m, 1 <= S m).
+            {
+              intros. induction m0.
+              - reflexivity.
+              - apply le_S. apply IHm0.
+            }
+            apply H4.
+        }
+        rewrite H4 in H2. apply H2.
   }
   assert (B: forall c phi, verifies g q (!! ([[c]]# (!! phi))) -> verifies g q (<<c>>^ phi)).
   {
-    intros. 
+    simpl. intros.
+    apply not_all_ex_not in H. destruct H.
+    apply not_all_ex_not in H. destruct H.
+    unfold not in H.
+    exists x0. 
   }
